\section{Fourier Analysis}
\subsection*{CT FS}
$x(t)=x(t+T), \omega_0=\frac{2\pi}{T}$

$c_k=\frac 1 T \int_T x(t) e^{-jk\omega_0 t} \rd t$

$\tilde{x}(t)=\sum_{k=-\infty}^{+\infty} c_k e^{jk\omega_0 t}=\begin{cases}x(t)\\ \frac{x(t+)+x(t-)}2\end{cases}$
\subsubsection*{Real Signals}
When $c_k*=c_{-k}$\\
$\begin{aligned}
        x(t) & =\frac{a_0}{2} + \sum_{k=1}^{\infty} (a_k \cos(k\omega_0t)+b_k\sin(k \omega_0 t)) \\
             & =A_0+\sum_{k=1}^{\infty} A_k\cos(k\om_0 t+\phi_k)
    \end{aligned}$

$|c_k|^2=|c_{-k}|^2=\frac{a_k^2+b_k^2}{4}$

\subsubsection*{Examples}
$x(t)=a[u(t+\frac\tau 2) - u(t-\frac\tau 2)]$

$c_0=a\frac\tau T$

$c_k=\frac{a\tau}{T} Sa(\frac{k\om_0\tau}{2})$

$Sa(t)=\begin{cases}\frac{\sin(t)}{t}, t\ne 0\\1, t=0\end{cases}$

\subsubsection*{Parseval Theorem}

$\frac  1 T \int_T |x(t)|^2\rd t = \sum_k |c_k|^2=A_0^2+\frac 1 2\sum_{k\ge 1} A_k^2$

\subsubsection*{Properties}
$\mathcal{FS}\{x(t)\}=c_k,\mathcal{FS}\{x(t-t_0)\}=c_ke^{-jk\om_0 t_0}$\\
$\mathcal{FS}\{x(t)\}=c_k,\mathcal{FS}\{x^*(t)\}=c_{-k}*$\\
$x(t)= \sum \frac{c_k+c_{-k}*}{2}e^{jk\om_0t} + j \sum \frac{c_k-c_{-k}*}{2j}e^{jk\om_0t}$ \\
$\mathcal{FS}\{x(t)y(t)\}=\sum c_ld_{k-l}=c_k*d_k$\\
$\mathcal{FS}\{x'(t)\}=jk\om_0c_k$\\
$\mathcal{FS}\{y(t)\}=\int_0^{t}x(\tau)\rd \tau, (0<t<T), y(t)=y(t+T)$\\$y(t)=\sum_{k\ne 0} \frac{c_k}{jk\om_0}(e^{jk\om_0 t} - 1) + c_0t$

\subsection{DT FS}

$x[n] = x[n + N]$

$x[n]=\sum_{k=0}^{N-1} c_ke^{\frac{j2\pi k n}{N}}, 0\le n<N$

$c_k=\frac 1 N\sum_{l=0}^{N-1} x[l] e^{-\frac{j2\pi k l}{N}}=c_{k+N}$

\subsubsection*{Examples}

$x[n]=\begin{cases}1,|n|<=N_1\\0, N_1<|n|<=\frac N 2 \end{cases}, \\\mathcal{FS}\{x[n]\}=\begin{cases}\frac{\sin[(2\pi k / N)(N_1 + \frac 1 2)]}{N\sin(2\pi k / 2N)}, k\ne tN\\\frac{2N_1+1}{N}, k=tN\end{cases}$

$\mathcal{FS}\{e^{j\om_0 n}\} = \begin{cases}
    1,k=m+tN\\0, otherwise
\end{cases}, \om_0 = \frac{2\pi m}{N}$


\subsection{CT FT}

$X(j\om) = \int_{-\infty}^{\infty} x(t) e^{-j\om t} \rd t$

$x(t)=\frac{1}{2\pi} \int_{-\infty}^{\infty} X(j\om) e^{j\om t}\rd \om$
\subsubsection*{Examples}

$\mathcal{F}\{x(t) = a[u(t+\frac\tau2)-u(t-\frac\tau2)]\} =  a\tau Sa(\frac{\om\tau}{2})$

$\mathcal{F}\{x(t) = e^{-\alpha t} u(t), (\alpha>0)\}=\frac{1}{\alpha + j\om}$

$\mathcal{F}\{\delta(t)\}=1, \mathcal{F}\{1\}=2\pi\delta(\om)$

$\mathcal{F}\{e^{j\om_0t}\} = 2\pi\delta(\om-\om_0)$

$\mathcal{F}\{\text{sgn}(t)\} = \frac{2}{j\omega}$
\subsubsection*{Periodic Signals}

$x(t)=\sum_{k=-\infty}^{+\infty} c_k e^{jk\omega_0 t}$

$\mathcal{F}\{x(t)\}=\int_{-\infty}^{+\infty} \sum_{k=-\infty}^{+\infty} c_ke^{jk\om_0t} e^{-j\om t}\rd t$

$ = 2\pi \sum_{k=-\infty}^{+\infty} c_k \delta(\om - k \om_0)$

\subsubsection*{Parseval Theorem}

$\int_{-\infty}^{+\infty} |x(t)|^2\rd t = \frac{1}{2\pi} \int_{-\infty}^{+\infty} |X(j\om)|^2\rd \om$

\subsubsection*{Properties}

$\mathcal{F}\{x(t)\} = X(j\om), \mathcal{F}\{X(jt)\} = 2\pi x(j^2\om)$\\
$\mathcal{F}\{x(t-\tau)\} = X(j\om) e^{-j\om\tau}$\\
$\mathcal{F}\{x(\alpha t)\} = \frac{1}{|\alpha|}X(\frac{j\om}{\alpha})$\\
$\mathcal{F}\{x^*(t)\} = X^*(-j\om)$\\
$\mathcal{F}\{x'(t)\} = j\om X(j\om), \mathcal{F}\{tx(t)\} = j\frac{\rd X(j\om)}{\rd \om}$\\
$\mathcal{F}\{\int_{-\infty}^{t} x(\tau) \rd \tau\} = \frac{X(j\om)}{j\om} +\pi X(0)\delta(\om)$\\
$\mathcal{F}\{-\frac{x(t)}{jt} +\pi x(0)\delta(t)\} = \int_{-\infty}^{\om} X(j\eta) \rd \eta$\\
$\mathcal{F}\{x_1(t)*x_2(t)\} = X_1(j\om) X_2(j\om),$\\
$\mathcal{F}\{x_1(t)x_2(t)\} = \frac{1}{2\pi}X_1(j\om) * X_2(j\om)$
\subsection{DT FT}

$X(e^{j\om}) = \sum_n x[n] e^{-j\om n} = X(e^{j(\om + 2\pi)})$ (*)

$x[n] = \frac{1}{2\pi} \int_{2\pi} X(e^{j\om}) e^{j\om n} \rd \om$

\subsubsection*{Examples}

$\mathcal{F}\{[|n|\le N_1]\} = \frac{\sin{\om(N_1+\frac 1 2)}}{\sin(\frac{\om}{2})}$\\

$\mathcal{F}\{\frac{\sin(Wn)}{\pi n}\}=[u(\om+W)-u(\om-W)]$(Periodic, $T=2\pi$)
$x[n] = \begin{cases} 1, n\ge 0\\-1, n<0\end{cases}$

$\mathcal{F}\{x[n]\}=\frac{2}{1-e^{-j\om}}$

$\mathcal{F}\{u[n]\}=\frac{1}{1-e^{-j\om}} + \pi\sum_{k=-\infty}^{+\infty} \delta(\om - 2k\pi)$

$\mathcal{F}\{e^{j\om_0n}\} = \sum_{n=-\infty}^{+\infty} e^{-j(\om-\om_0)n} = 2\pi\sum \delta(\om-\om_0-2k\pi)$

\subsubsection*{Periodic Signals}

$x[n] = x[n+N]$, Fourier Series $x[n] = \sum_{k=0}^{N-1} c_k e^{\frac{j2\pi k n}{N}}$\\
$c_k = \frac{1}{N} \sum x[l] e^{\frac{-j2\pi k l}{N}} = c_{k + N}$\\
$\mathcal{F}\{x(t)\} = \sum_{k = 0}^{N - 1} c_k\mathcal{F}\{e^{\frac{j2\pi kn}{N}}\}=\sum_{k=-\infty}^{+\infty} 2\pi c_k\delta(\om-\frac{2k\pi}{N})$

\subsubsection*{CT FS and DT FT}

$X(e^{j\om}) = \sum_n x[n] e^{-j\om n} = X(e^{j(\om + 2\pi)})$\\
$x[n] = \frac{1}{2\pi} \int_{2\pi} X(e^{j\om}) e^{j\om n} \rd \om$\\
$c_k=\frac 1 T \int_T x(t) e^{-jk\omega_0 t} \rd t$\\
$x(t)=\sum_{k=-\infty}^{+\infty} c_k e^{jk\omega_0 t}$

$x[n]=c_{-n}\rightarrow x(t)=X(e^{j\om_0 t})$

\subsubsection*{Properties}

$x_k[n] = \begin{cases}x[n/k], n/k\in Z\\0, otherwise \end{cases}$\\
$\mathcal{F}\{x_k[n]\} = X(e^{jk\om})$\\
$\mathcal{F}\{x[n] - x[n - 1]\} = (1-e^{-j\om}) X(e^{jk\om})$\\
$\mathcal{F}\{nx[n]\} = j\frac{\rd X(e^{j\om})}{\rd \om}$\\
$\mathcal{F}\{\sum_{k\le n} x[k]\} = \frac{X(e^{j\om})}{(1-e^{-j\om})} + \pi X(e^{j0}) \sum \delta(\om - 2k\pi)$\\
$\mathcal{F}\{x[n]y[n]\}=\frac{1}{2\pi} \int_{2\pi} X(e^{j\theta})Y(e^{j(\om-\theta)})\rd \theta$

\subsection{DFT}

$X[k]=X(e^{\frac{j2\pi k}{N}})$ (sampling DT FT)